\documentclass[12pt]{article}
\usepackage[utf8]{inputenc}
\usepackage[english]{babel}
\usepackage{amssymb}
\usepackage{graphicx}
\usepackage{float}
\graphicspath{ {images/} }

\textwidth=431pt
\textheight=600pt
\hoffset=-30pt
\voffset=-30pt

\usepackage{graphicx}
\usepackage{amsmath}
\makeatletter
\renewcommand{\@oddhead}{
	\vbox{
		\hbox to \textwidth{\strut \textit{Think Math, Problem set 5, Usvyatsov Mikhail} \hfill }
		\hrule
		\vspace{12pt}
	}
}
\renewcommand{\@oddfoot}{}
\makeatother
	
	
\begin{document}
	\begin{center}
		\textbf{Problem set 5\\ Usvyatsov Mikhail}
	\end{center}
		
	\bigskip
	
	\textbf{Problem 1}
	
	\medskip
	$MI(X, Y) = H(Y) - H(Y|X) = - \sum_{y}p(y)ln(p(y)) + \sum_{x}p(x)\sum_{y}p(y|x)ln(p(y|x)) =$\\
	$=- \sum_{y}p(y)ln(p(y)) + \sum_{x, y}p(y|x)p(x)ln(p(y|x)) =  \sum_{x, y}p(x, y)ln(\frac{p(x, y)}{p(x)}) - \sum_{y}p(y)ln(p(y))=$\\
	$=\sum_{x, y}p(x, y)ln(\frac{p(x, y)}{p(x)}) - \sum_{x, y}p(y|x)ln(p(y))= \sum_{x, y}p(x, y)ln\left(\frac{p(x, y)}{p(x)p(y)}\right)$\\
	The last formula is exactly $KL(p||g)$. QED.
	\bigskip

	\textbf{Problem 2}
	
	\medskip
	
	$K(x, z) = e^{-\gamma || x - z ||^2}$
	
	According to Merser's theorem function k is a kernel iff:
	
	\begin{enumerate}
		\item
			K(x, z) = K(z, x), that obviously holds in our case.
		\item
			$\int_x\int_z K(x, z) g(x)g(z) dx dz \geq 0$ for every function g: X $\rightarrow$ R
	\end{enumerate}
	
	To prove the second condition is quite difficult.
	
	Instead of this we can see that:
	
	$e^{-\gamma || x - z ||^2} = \sum_{k=0}^{\infty} \frac{(2 \gamma <x, z>)^k}{k!}$
	
	That is the sum of products of kernels $2 \gamma <x, z>$.
	According to the materials of lecture 9 $<x, z>$ is a valid Mercer Kernel.
	
	Due to the fact that given two Mercer kernels its multiplication is also a Mercer Kernel and its sum is also a valid Mercer Kernel. QED.
	
	\medskip
	
	\textbf{Problem 3}
	\medskip
	
	$\omega_i^{m+1} = \frac{\omega_i^m e^{-\alpha_m y_i h^m(x_i)}}{Z_m}$
	
	$\sum_{i} \omega_i^{m+1} = 1$
	
	From previous we can derive:
	$Z_m = \sum_{i} \omega_i^{m+1} = \sum_i \omega_i^m e^{-\alpha_m y_i h^m(x_i)} = \sum_{correct} \omega_i^m e^{-\alpha_m y_i h^m(x_i)} + \sum_{incorrect} \omega_i^m e^{-\alpha_m y_i h^m(x_i)} = \epsilon_m  e^{\alpha_m} + (1 - \epsilon_m)e^{-\alpha_m}$, where $\alpha_m = \frac{1}{2} log\left( \frac{1-\epsilon_m}{\epsilon_m} \right)$
	
	Then updated error rate is $\epsilon_{m+1} = \sum_{incorrect} \omega_i^{m + 1} = \sum_{incorrect} \frac{\omega_i^m e^{-\alpha_m y_i h^m(x_i)}}{Z_i} = \sum_{incorrect} \frac{\omega_i^m e^{-\alpha_m}}{Z_i} = \frac{1}{2}$
	\medskip
\end{document}